Otway-Rees: refined mutual authentication properties to include timeliness
The proof for authentication in both ways includes a "triangular relation"
between the initiator/responder nonce which has to match over the course of
two events for the same principal and the conversation id which has to match
for the 'initiate' and 'request key' events.

otway-rees-fixed/OYRS.Messages.fsti
@@ -68,10 +68,10 @@ let event_request_key (c:bytes) (a b srv:principal) (n_b:bytes) : event =
   ("req_key",[c;(string_to_bytes a);(string_to_bytes b);(string_to_bytes srv);n_b])
 let event_send_key (c:bytes) (a b srv:principal) (n_a n_b k_ab:bytes) : event =
   ("send_key",[c;(string_to_bytes a);(string_to_bytes b);(string_to_bytes srv);n_a;n_b;k_ab])
-let event_forward_key (c:bytes) (a b srv:principal) (k_ab:bytes) : event =
-  ("fwd_key",[c;(string_to_bytes a);(string_to_bytes b);(string_to_bytes srv);k_ab])
-let event_recv_key (c:bytes) (a b srv:principal) (k_ab:bytes) : event =
-  ("recv_key",[c;(string_to_bytes a);(string_to_bytes b);(string_to_bytes srv);k_ab])
+let event_forward_key (c:bytes) (a b srv:principal) (n_b k_ab:bytes) : event =
+  ("fwd_key",[c;(string_to_bytes a);(string_to_bytes b);(string_to_bytes srv);n_b;k_ab])
+let event_recv_key (c:bytes) (a b srv:principal) (n_a k_ab:bytes) : event =
+  ("recv_key",[c;(string_to_bytes a);(string_to_bytes b);(string_to_bytes srv);n_a;k_ab])
 
 
 let oyrs_key_usages : LC.key_usages = LC.default_key_usages
