otway-rees-fixed/OYRS.SecurityProps.fsti
@@ -145,16 +145,28 @@ val conv_key_stored_in_responder_state_is_secret:
     )
   ))
 
+/// Ensures initiator authentication.
+/// This property ensures that for every 'forward key' event, there are preceding 'initiate' (triggered by initiator) and 'request key' events with the same
+/// conversation id such that the responder nonce from the 'forward key' event
+/// matches with the one from the 'request key' event.
+/// This leads to the conclusion that there was a timely initiation of the protocol
+/// from the initiator targeting the responder, confirming the believes of the
+/// responder.
 val initiator_authentication: i:nat ->
   LCrypto unit (pki oyrs_preds)
   (requires (fun t0 -> i < trace_len t0))
-  (ensures (fun t0 _ t1 -> forall c a b srv k_ab.
-  did_event_occur_at i b (event_forward_key c a b srv k_ab)
-  ==> ((exists c n_a. did_event_occur_before i a (event_initiate c a b srv n_a)) \/ corrupt_id i (P a) \/ corrupt_id i (P b) \/ corrupt_id i (P srv))))
+  (ensures (fun t0 _ t1 -> forall c a b srv n_b k_ab.
+  did_event_occur_at i b (event_forward_key c a b srv n_b k_ab)
+  ==> ((exists c' n_a. did_event_occur_before i a (event_initiate c' a b srv n_a)
+    /\ did_event_occur_before i b (event_request_key c' a b srv n_b))
+    \/ corrupt_id i (P a) \/ corrupt_id i (P b) \/ corrupt_id i (P srv))))
 
+/// Ensures responder authentication analogous to initiator authentication
 val responder_authentication: i:nat ->
   LCrypto unit (pki oyrs_preds)
   (requires (fun t0 -> i < trace_len t0))
-  (ensures (fun t0 _ t1 -> forall c a b srv k_ab.
-  did_event_occur_at i a (event_recv_key c a b srv k_ab)
-  ==> ((exists c n_b. did_event_occur_before i b (event_request_key c a b srv n_b)) \/ corrupt_id i (P a) \/ corrupt_id i (P b) \/ corrupt_id i (P srv))))
+  (ensures (fun t0 _ t1 -> forall c a b srv n_a k_ab.
+  did_event_occur_at i a (event_recv_key c a b srv n_a k_ab)
+  ==> ((exists c' n_b. did_event_occur_before i b (event_request_key c' a b srv n_b)
+    /\ did_event_occur_before i a (event_initiate c' a b srv n_a))
+    \/ corrupt_id i (P a) \/ corrupt_id i (P b) \/ corrupt_id i (P srv))))
